new.dfy
@@ -1,0 +1,136 @@
+class {:autocontracts} FilaCircular {
+  var fim: nat;
+  var inicio: nat;
+  var a: array<nat>;
+  var tamanho: nat;
+
+  ghost var Conteudo: seq<nat>;
+
+  ghost predicate Valid() {
+    (0 <= inicio < a.Length) &&
+    (0 <= fim < a.Length) &&
+    (a.Length > 0) &&
+    ((fim >= inicio ==> Conteudo == a[inicio..fim]) ||
+    (fim < inicio ==> Conteudo ==  a[inicio..] + a[0..fim])) &&
+    (tamanho == |Conteudo|)
+    }
+
+    constructor()
+      ensures Conteudo == []
+      ensures inicio == 0
+      ensures fim == 0
+      ensures a.Length == 5
+      ensures a.Length == 5
+    {
+    inicio := 0;
+    fim := 0;
+    a:= new nat[5];
+    Conteudo := [];
+    tamanho := 0;
+    }
+
+  method enqueue(e: nat)
+    ensures Conteudo == old(Conteudo) + [e]
+  {
+    // if (tamanho == a.Length) {
+    //   var novoA := new nat[2 * a.Length];
+
+    //   var i := 0;
+
+    //   while i < a.Length
+    //     invariant novoA.Length > a.Length
+    //     invariant novoA.Length > inicio
+    //     invariant fim == old(fim)
+    //     invariant Conteudo == old(Conteudo)
+    //     invariant fresh(novoA)
+    //   {
+    //     var item := a[i];
+    //     novoA[i] := item;
+    //     i := i + 1;
+    //   }
+
+    //   a := novoA;
+    // }
+
+    a[fim] := e;
+    fim := (fim + 1) % a.Length;
+    Conteudo := Conteudo + [e];
+    tamanho := tamanho + 1;
+  }
+
+  method contains(element: nat) returns (b: bool)
+    requires |Conteudo| > 0
+    requires fim != inicio
+    // ensures b <==> exists i :: 0 <= i < |Conteudo| && element == Conteudo[i]
+  {
+    var i := inicio;
+    var iterations := 0;
+    b := false;
+
+    // [1, , 2, 3] -- inicio 2, cauda 1 --> size 3
+    // [2, 3, 1]
+    // it = 0, i = 2
+    // it = 1, i = 3
+    // it = 2, i = 0
+    // retorna
+
+
+    // [, , 1, 2, 3] -- inicio 2, fim 3 --> size 3
+    // [1, 2, 3]
+    // it = 0, i = 2
+    // it = 1, i = 3
+    // it = 2, i = 4
+    // retorna
+
+    while iterations < tamanho
+      invariant tamanho == |Conteudo|
+      invariant 0 <= iterations <= tamanho
+      invariant fim == old(fim)
+      invariant inicio == old(inicio)
+      invariant Conteudo == old(Conteudo)
+      invariant fim > inicio && iterations > 0 ==> (inicio <= i <= fim < a.Length) && ((i - iterations) == (i - 1))
+      invariant fim >= inicio ==> inicio <= i <= fim
+
+      invariant ((fim >= inicio ==> Conteudo == a[inicio..fim]) ||
+                (fim < inicio ==> Conteudo ==  a[inicio..] + a[0..fim]))
+
+      // invariant forall j: nat :: j < iterations ==> Conteudo[j] != element
+    {
+      if a[i] == element {
+        // assert Conteudo[iterations] == element;
+        b := true;
+        return;
+      }
+      var i := (i + 1) % a.Length;
+      iterations := iterations + 1;
+    }
+  }
+}
+
+method Print(fila: FilaCircular) {
+  print("\n\n");
+  var i := 0;
+  while i < fila.a.Length{
+    print(fila.a[i]);
+    print("  ");
+    i := i + 1;
+  }
+}
+
+
+method Main() {
+  var fila := new FilaCircular();
+  fila.enqueue(1);
+  fila.enqueue(2);
+  fila.enqueue(3);
+  fila.enqueue(4);
+  fila.enqueue(5);
+  assert fila.Conteudo == [1, 2, 3, 4, 5];
+
+  assert fila.Conteudo[0] == 1;
+  assert fila.a[0] == 1;
+  var contem := fila.contains(1);
+  assert contem == true;
+
+  Print(fila);
+}
