something.dfy
@@ -1,0 +1,124 @@
+class {:autocontracts} CircularQueue
+    {
+    var elements: array<int>;
+    var front: int;
+    var count: int;
+    const defaultSize: nat;
+
+
+    constructor ()
+    ensures front == 0
+    ensures count == 0
+    ensures elements.Length >= defaultSize
+    ensures defaultSize == 5
+    ensures fresh(elements)
+    {
+    elements := new int[5];
+    front := 0;
+    count := 0;
+    defaultSize := 5;
+    }
+
+    ghost predicate Valid()
+    reads this
+    {
+                        //   0 <= count <= elements.Length &&
+     0 <= front < elements.Length
+    }
+
+  method Enqueue(element: int)
+    ensures count == old(count) + 1
+    {
+    if count == elements.Length {
+      var newElements := new int[2 * elements.Length];
+      for i: int := 0 to elements.Length - 1
+        invariant elements.Length > 0
+        invariant count == old(count)
+    {
+        var index := (front + i) % elements.Length;
+        newElements[i] := elements[index];
+    }
+      elements := newElements;
+      front := 0;
+    }
+
+    var rear := (front + count) % elements.Length;
+    elements[rear] := element;
+    count := count + 1;
+    }
+
+  method Dequeue() returns (element: int)
+    requires count > 0
+  {
+    element := elements[front];
+    front := (front + 1) % elements.Length;
+    count := count - 1;
+  }
+
+  function Size(): int
+  {
+    count
+  }
+
+  method Contains(element: int) returns (b: bool)
+    requires elements.Length > 0
+  {
+    var i := front;
+    var iterations := 0;
+    b := false;
+
+    while iterations < count
+      invariant iterations <= count
+      invariant 0 <= i < elements.Length
+    {
+      if elements[i] == element {
+        b := true;
+        return;
+      }
+
+      i := (i + 1) % elements.Length;
+      iterations := iterations + 1;
+    }
+  }
+
+  method Concat(queue: CircularQueue) returns (newQueue: CircularQueue)
+    requires queue.Valid()
+    requires queue.Size() > 0
+    requires Size() > 0
+    ensures newQueue.Valid()
+    ensures newQueue.Size() == Size() + queue.Size()
+  {
+    newQueue := new CircularQueue();
+
+    var thisSize := Size();
+    var queueSize := queue.Size();
+
+    assert newQueue.Size() == 0;
+
+    // Copia o conteúdo da fila atual para newQueue
+    for i: int := 0 to thisSize - 1
+      invariant newQueue.count == i
+      //   invariant i <= newQueue.elements.Length
+      invariant fresh(newQueue.Repr)
+      //   invariant Size() == thisSize - i
+    {
+      var index := (front + i) % elements.Length;
+      var element := elements[index];
+      newQueue.Enqueue(element);
+    }
+
+    // Copia o conteúdo da fila queue para newQueue
+    for i: int := 0 to queueSize - 1
+      invariant newQueue.Size() == thisSize + i
+      invariant queue.Size() == queueSize - i
+    {
+      var index := (queue.front + i) % queue.elements.Length;
+      var element := queue.elements[index];
+      newQueue.Enqueue(element);
+    }
+
+    return newQueue;
+  }
+
+
+}
